Clean examples.

src/Narcissus/Examples/PermutationOpt.v
@@ -96,12 +96,12 @@ Module SimplPermutation.
   Let encode := encoder_impl enc_dec.
   
   Let decode := decoder_impl enc_dec.
-  Print Assumptions decode.
+  Print Assumptions enc_dec.
 
 
 End SimplPermutation.
 
-Module TopPermutation.
+Module FourPermutation.
   (* Just like a SimplPermutation, but encodes five elements. *)
 
   Let types:= [word 8:Type; word 16:Type; word 32:Type; word 64:Type].
@@ -151,596 +151,71 @@ Module TopPermutation.
   Let decode := decoder_impl enc_dec.
   Print Assumptions decode.
 
-  Goal forall m b x, decode m b  = x.
-    unfold decode.
+  
+End FourPermutation.
+
+
+Module AllEqualPermutation.
+  (* Just like a SimplPermutation, but encodes five elements. *)
+
+  Let types:= [word 8:Type; word 8:Type; word 8:Type; word 8:Type].
+  
+  Let invariants := ilist_constant_T types.
+  Let view_fin {n} (f:Fin.t n):= f2n f < pow2 8.
+  Let invariant := (fun st : SumType types =>
+                      view_fin (SumType_index types st) /\
+                        ith invariants (SumType_index types st) (SumType_proj types st)).
+
+  Record message := {
+      label1 : word 8
+    ; label2 : word 8
+    ; label3 : word 8
+    ; label4 : word 8                   
+    }.
+
+  Let myProjections: ilist (B:=fun T => _ -> T) types := {{ label1 ; label2 ; label3 ; label4 }}.
+  Let myTypes {n: nat} {types: Vector.t Type n} {B} (list: ilist (B:=B) types): Vector.t Type n:= types.
+  
+  Let myCodes: Vector.t (word 8) 4:= [[ natToWord _ 1; natToWord _ 3; natToWord _ 4; natToWord _ 7 ]].
+  Let myFinFormat:= (format_enum myCodes).
+  
+  Let myFormats: ilist (B := fun T => FormatM T ByteString) (myTypes myProjections)
+      := {{ format_word; format_word; format_word; format_word }}.
+  
+  Ltac new_encoder_rules ::=
+    eapply Permutation_Encoder_Correct;
+    [| unfold Vector.nth; repeat constructor | |IndexedSumType.split_iterate ]; simpl;
+    eauto with resilience.
+
+  Definition inv (msg: message):= True.
+
+  Definition myFormat:= permutation_Format myProjections myFinFormat myFormats.
+    
+  Let enc_dec : EncoderDecoderPair myFormat inv.
+  Proof.
+    unfold myFormat, myFinFormat.
+    derive_encoder_decoder_pair.
+    
+    Unshelve.
+    constructor.
+  Defined.
 
   
-End TopPermutation.
+  Let encode := encoder_impl enc_dec.
   
-
-
-
-
-
-
-
-
-
-
-
-
-
-
-
-
-
-
-
-
-
-
-
-
-
-
-
-          
-          
-          (** * Old  version. *)
-          (* This version builds the format from scratch. Great for exploration.
-
-TODO: DELETE when the rest is ready!
-           *)
-          
-          Module PermutationCodes2.  
-        Let types:= [word 8:Type; word 16:Type].
-
-        Let myTuple:= ituple types.
-
-        Definition formats : ilist (B := fun T => FormatM T ByteString) types
-          := {{ format_word; format_word }}.
-        
-        Let invariants := ilist_constant_T types.
-        Let view_fin {n} (f:Fin.t n):= f2n f < pow2 8.
-        Let invariant := (fun st : SumType types =>
-                            view_fin (SumType_index types st) /\ ith invariants (SumType_index types st) (SumType_proj types st)).
-
-        Definition lift_SumType (A:Type) {n:nat} {types:Vector.t Type n} :
-          SumType types -> SumType (Vector.cons Type A _ types):=
-          match types as typs return
-                SumType typs -> SumType (Vector.cons Type A _ typs) with
-          | Vector.nil =>
-              (* Impossible case: with an empty vector can't construct the SumType*)
-              fun elem => let X1 := match elem return A with
-                                    end in X1
-          | Vector.cons a n typs' =>
-              fun elem => inr elem
-          end.
-        
-        Fixpoint to_list {n:nat} {S:Type} {types:Vector.t Type n}:
-          forall projections: ilist (B:= fun T => S -> T) types, 
-            S -> list (SumType types):=
-          match types as typs return
-                ilist (B:= fun T => S -> T) typs ->  
-                S -> list (SumType typs) with
-          | Vector.nil => fun _ _ => Datatypes.nil
-          | @Vector.cons _ a n' typs' =>
-              let typs:= Vector.cons Type a n' typs' in
-              fun projs S =>
-                (inj_SumType typs Fin.F1 (prim_fst projs S))
-                  :: map (lift_SumType a) (to_list (prim_snd projs) S)
-          end.
-
-        Definition format_SumType_list
-          (m : nat) (types : Vector.t Type m)
-          (fin_format: FormatM (Fin.t m) ByteString)
-          (formats: ilist (B:= fun T => FormatM T ByteString) types):
-          FormatM (list (SumType types)) ByteString:=
-          format_list (format_IndexedSumType m types formats fin_format).
-
-        
-        Definition format_permutation_list
-          (m : nat) (types : Vector.t Type m)
-          (fin_format: FormatM (Fin.t m) ByteString)
-          (formats: ilist (B:= fun T => FormatM T ByteString) types):
-          FormatM (list (SumType types)) ByteString:=
-          Compose_Format (format_SumType_list m types fin_format formats)
-            (Permutation (A:=SumType types)).
-        
-        
-        
-        Definition format_through_list
-          S
-          (m : nat) (types : t Type m)
-          (projections: ilist (B:= fun T => S -> T) types)
-          (fin_format: FormatM (Fin.t m) ByteString)
-          (formats: ilist (B:= fun T => FormatM T ByteString) types):
-          FormatM S ByteString:=
-          format_permutation_list m types fin_format formats ◦ to_list projections.
-        
-        Record message := {
-            label : word 8
-          ; data : word 16                     
-          }.
-
-        Let myProjections: ilist (B:=fun T => _ -> T) types := {{ label ; data }}.
-        Let myTypes {n: nat} {types: Vector.t Type n} {B} (list: ilist (B:=B) types): Vector.t Type n:= types.
-        
-        Let myCodes: Vector.t (word 8) 2:= [[ natToWord _ 42; natToWord _ 73 ]].
-        Let myFinFormat:= (format_enum myCodes).
-        
-        Let myFormats: ilist (B := fun T => FormatM T ByteString) (myTypes myProjections) := {{ format_word; format_word }}.
-        
-        Let myFormat:= format_through_list message _ types myProjections myFinFormat myFormats.
-        
-        Let enc_dec : EncoderDecoderPair myFormat (constant True).
-        Proof.
-          (*unfold myFormat,format_through_list, format_permutation_list.*)
-          (* derive_encoder_decoder_pair. *)
-          econstructor.
-          - (* synthesize_aligned_encoder. *)
-            start_synthesizing_encoder.
-            normalize_encoder_format.
-            
-            align_encoder_step. (*splits emty*)
-            align_encoder_step. (* removes empty*)
-            (*eapply CorrectAlignedEncoderProjection.*)
-            align_encoder_step. (*projection*)
-            
-            unfold format_permutation_list.
-            match goal with
-              |- CorrectAlignedEncoder (Compose_Format ?X _) ?enc =>
-                cut (CorrectAlignedEncoder X enc) 
-            end.
-            + (*This should be trivial, since identity is a premutation*)
-              unfold format_SumType_list.
-              shelve.
-            + repeat align_encoder_step.
-          - (* synthesize_aligned_decoder. *)
-            start_synthesizing_decoder.
-            + Lemma EquivFormat_compose_projection {T S S' S''}
-                (format_S'' : FormatM S'' T)
-                (f : S -> S')
-                (r : S' -> S'' -> Prop)
-                : EquivFormat (Projection_Format (Compose_Format format_S'' r) f)
-                    (Compose_Format format_S'' (fun a b => r (f a) b)).
-              Proof.
-                unfold EquivFormat, refineEquiv, Projection_Format, Compose_Format, compose, Bind2; split;
-                  intros ? ?.
-                - rewrite unfold_computes in *.
-                  destruct_ex; split_and; eexists.
-                  rewrite unfold_computes;  eauto.
-                - rewrite unfold_computes in *.
-                  destruct_ex; split_and.
-                  rewrite unfold_computes in H0.
-                  destruct_ex; split_and.
-                  eexists; intuition eauto.
-                  subst; eauto.
-              Qed.
-
-              Ltac normalize_step BitStringT ::=
-                (first_debug
-                   [ match goal with
-                     | |- EquivFormat ?z ?x => is_evar z; apply EquivFormat_reflexive
-                     end; idtac "1"
-                   | eapply EquivFormat_trans; [ apply sequence_assoc |  ]
-                     ; idtac "3"
-                   | eapply EquivFormat_trans;
-                     [ apply sequence_mempty with (monoid := BitStringT) |  ]
-                     ; idtac "5"
-                   | eapply EquivFormat_ComposeIf; intros
-                     ; idtac "6"
-                   | eapply EquivFormat_trans;
-                     [ apply EquivFormat_If_Then_Else with (monoid := BitStringT) |  ]
-                     ; idtac "8"
-                   | apply EquivFormat_If_Then_Else_Proper
-                     ; idtac "9"
-                   | eapply EquivFormat_UnderSequence';
-                     [ repeat
-                         (eapply EquivFormat_trans;
-                          [ first [eapply EquivFormat_compose_map; idtac "10.0" |
-                                    eapply EquivFormat_compose_projection; idtac "10.1" ] |  ] );
-                       apply EquivFormat_reflexive
-                     |  ] ; idtac "10"
-                   | eapply EquivFormat_Projection_Format_Empty_Format';
-                     [ repeat eapply EquivFormat_compose_map;
-                       apply EquivFormat_reflexive ] ; idtac "11"
-                   | unfold EquivFormat; intros; reflexivity ]); 
-                intros.
-              normalize_format. 
-              eapply sequence_Compose_format_decode_correct; cycle 1.
-              * unfold format_SumType_list.
-                unfold myFinFormat.
-                (*1*) intros; apply FixList_decode_correct.
-                apply_IndexedSumType_Decoder_Correct 2 types.
-                unfold Vector.nth; simpl; eapply H.
-                simpl;
-                  repeat
-                    match goal with
-                    | |- IterateBoundedIndex.prim_and _ _ =>
-                        apply
-                          IterateBoundedIndex.Build_prim_and
-                    end; try exact I; simpl; 
-                  intros.
-                3: intros.
-
-                intuition
-                  eauto
-                    2
-                  with data_inv_hints.
-                2: { unfold Vector.nth; simpl; eapply H.
-                     | .
-                     simpl;
-                       repeat
-                         match goal with
-                         | |- IterateBoundedIndex.prim_and _ _ =>
-                             apply IterateBoundedIndex.Build_prim_and
-                         end; try exact I; simpl; intros. ].
-                
-                apply_rules.
-                
-              * intuition; split; try reflexivity.
-                etransitivity.
-                symmetry; eapply Permutation_length; eauto.
-                simpl; reflexivity.
-                intros ?.
-                match goal with
-                | |-
-                    context [ fun st b' =>
-                                ith _ (SumType_index _ st) (SumType_proj _ st) b' ] =>
-                    let a'' := fresh in
-                    intro a''; intros;
-                    repeat instantiate ( 1 := (constant (constant True)) );
-                    repeat destruct a'' as [?| a'']; auto
-                | |-
-                    context [ fun st b' =>
-                                ith _ (SumType_index _ st) (SumType_proj _ st) b' ] =>
-                    let a'' := fresh in
-                    intro a''; intros;
-                    repeat instantiate ( 1 := (constant (constant True)) );
-                    repeat destruct a'' as [?| a'']; auto
-                end.
-                
-                solve_side_condition.
-                
-                intros; split; auto.
-                admit.
-                shelve.
-              * (*ExtractSource. *)
-                simpl; intros; eapply CorrectDecoderEmpty.
-                -- unfold Heading.Domain, Tuple.GetAttribute, Tuple.GetAttributeRaw,
-                     Basics.compose in *; simpl in *.
-                   let a' := fresh in
-                   intros a'; try destruct a'; destruct_conjs.
-                   unfold Heading.Domain, Tuple.GetAttribute, Tuple.GetAttributeRaw in *;
-                     simpl in *; intros. decompose_source_predicate. subst_projections.
-                   Require Import Sorting.Sorting.
-                   Definition sort: forall A, list A -> list A.
-                   Admitted.
-
-                   
-                   Definition smart_head {A:Type} (ls: list A): (|ls|) > 0 -> A:=
-                     match ls as l return ((| l |) > 0 -> A) with
-                     | []%list => fun H : 0 > 0 => ltac:(lia)
-                     | a :: ls0 => constant a
-                     end.
-                   Definition smart_tail {A:Type} (ls: list A): (|ls|) > 0 -> list A:=
-                     match ls as l return ((| l |) > 0 -> list A) with
-                     | []%list => fun H : 0 > 0 => ltac:(lia)
-                     | a :: ls0 => constant ls0
-                     end.
-
-                   Lemma smart_list_split_witness:
-                     forall {A ls ls'} {x:A} (H: (x::ls')%list = ls),
-                       (|ls|) > 0.
-                   Proof.
-                     intros. destruct ls; simpl in *; try discriminate.
-                     unfold ">".
-                     lia.
-                   Qed.
-                   Lemma smart_list_split:
-                     forall A ls ls' (x:A) (H: (x::ls')%list = ls),
-                       x = smart_head ls (smart_list_split_witness H) /\
-                         ls' = smart_tail ls (smart_list_split_witness H).
-                   Proof. intros; split; subst ls; reflexivity. Qed.
-                   
-                   
-                   Instance Permutation_ConditionallyInvertibleRel {n}{types: Vector.t Type n}:
-                     ConditionallyInvertibleRel (@Permutation (SumType types))
-                       (fun a => Sorted eq a) (sort (SumType types)).
-                   Proof.
-                     constructor.
-                     intros.
-                   Admitted.
-
-                   Print Instances ConditionallyInvertibleRel.
-                   eapply CInvRoundTripRel in H0.
-                   Ltac blah:= match goal with
-                               | [H: (?a::?ls')%list = ?x |- _ ] =>
-                                   let HH:= fresh "HH" in
-                                   idtac H;
-                                   pose proof (smart_list_split _ _ _ _ H) as HH;
-                                   try clear H; destruct HH
-                               end.
-                   blah.
-                   blah.
-                   Definition inv_inr: (
-                                         clear H0.
-                     
-                     
-                     
-                     2: { admit. }
-
-                     Ltac blah:=
-                       match goal with
-                       | [H: (?a::?ls')%list = ?x |- _ ] => 
-                           let HH:= fresh "HH" in
-                           destruct x eqn:HH; try discriminate;
-                           injection H; try clear H;
-                           let H':=fresh in
-                           let Hnew_eq:= fresh "Hnew_eq" in
-                           intros H' Hnew_eq
-                       | [H: ([])%list = ?x |- _ ] =>
-                           subst x
-                       end.
-
-                     repeat blah.
-                     
-
-                     unshelve instantiate(1:=_).
-                     
-                     
-                     
-                     match goal with
-                     | H:?f ?x ?y
-                       |- _ =>
-                         eapply CInvRoundTripRel in H;
-                         [  | now typeclasses eauto | now simpl in *; eauto ]; 
-                         try subst x
-                     end.
-                     
-                     Lemma Permutation_remove
-                             
-                             
-                       subst_invertible. reflexivity).
-
-
-                   | decide_data_invariant ] ].
-
-                                              
-                                              
-                                              lazymatch goal with
-                                                |- CorrectDecoder ?mon _ _ _ (Compose_Format ?YY ?R ++ _) _ _ _ =>
-                                                  remember YY as XX
-                                              end.
-                                              exploit @sequence_Compose_format_decode_correct.
-                                              5:{ intros HH.
-                                                  match type of HH with
-                                                    CorrectDecoder ByteStringQueueMonoid ?Goal11 
-                                                      ?Goal11 eq (Compose_Format ?Goal13 ?Goal10 ++ ?Goal14)
-                                                      (sequence_Decode ?Goal15 ?Goal18) ?Goal6
-                                                      (Compose_Format ?Goal13 ?Goal10 ++ ?Goal14) =>
-                                                      unify Goal11 ((fun _ : message => True));
-                                                      try unify Goal13 XX;
-                                                      unify Goal10 (fun (a' : message) (b' : list (SumType types)) =>
-                                                                      Permutation [inl (label a'); inr (data a')] b') 
-                                                  end.
-                                                  revert HH.
-                                                  lazymatch goal with
-                                                    |- CorrectDecoder ByteStringQueueMonoid (constant True) 
-                                                         (constant True) eq
-                                                         (Compose_Format XX
-                                                            (fun (a' : message) (b' : list (SumType types)) =>
-                                                               Permutation [inl (label a'); inr (data a')] b') ++ 
-                                                            ?Goal9) ?Goal10 ?Goal4
-                                                         (Compose_Format XX
-                                                            (fun (a' : message) (b' : list (SumType types)) =>
-                                                               Permutation [inl (label a'); inr (data a')] b') ++ 
-                                                            ?Goal9) ->
-                                                       CorrectDecoder AlignedByteString.ByteStringQueueMonoid 
-                                                         (constant True) (constant True) eq
-                                                         (Compose_Format XX
-                                                            (fun (a' : message) (b' : list (SumType types)) =>
-                                                               Permutation [inl (label a'); inr (data a')] b') ++ ?empty_Format)
-                                                         ?decoder ?cache_inv
-                                                         (Compose_Format XX
-                                                            (fun (a' : message) (b' : list (SumType types)) =>
-                                                               Permutation [inl (label a'); inr (data a')] b')) =>
-                                                      unify decoder Goal10;
-                                                      unify cache_inv Goal4
-                                                  end.
-                                                  unshelve instantiate(4:=_). eapply empty_Format.
-                                                  intros HH. eapply HH.
-                                                  
-                                                  eapply HH.
-                                                  unshelve instantiate(2:= _) in HH.
-                                                  
-                                                  eapply HH.
-                                                  unfold "◦".
-                                                  eapply (format_sequence_correct H) with (monoid :=  AlignedByteString.ByteStringQueueMonoid ).
-                                                  * clear H; intros; apply_rules.
-                                                    
-                                                    exploit @Compose_decode_correct.
-                                                    3: { intros HH.
-                                                         match type of HH with
-                                                           CorrectDecoder ?mon ?g9 ?g10 ?g8 (Compose_Format ?g11 ?g8) ?g13 ?g7 ?g12 =>
-                                                             unify g9 g10;
-                                                             unify g8 eq;
-                                                             unify g11
-                                                         end.
-                                                         
-                                                         
-                                                         * clear H. (*solve [ solve_side_condition ].*) shelve.
-                                                         * clear H; intros; apply_rules.
-
-                                                           apply_rules.
-                                                         + cbv beta; synthesize_cache_invariant.
-                                                         + cbv beta; unfold decode_nat, sequence_Decode; optimize_decoder_impl.
-                                                         + cbv beta; align_decoders.
-                                                           
-
-                                                           
-                                                           Unshelve.
-                                                           (* This one is due to way `align_decoders_step`  deals with
-       `IterateBoundedIndex.prim_and`.
-       There is an already shelved `ilist` that slowly
-       decreases but obviously never gets completed (since the last goal doesn't depend).
-                                                            *)
-                                                           constructor.
-                                              Defined.
-                                              
-                                              Let encode := encoder_impl enc_dec.
-                                              
-                                              Let decode := decoder_impl enc_dec.
-                                              Print Assumptions decode.
-                                              
-                                              End SumTypeCodes2.
-
-                                              (** * Repeated type*)
-                                              (* | In this module show that IndexedSumType, by virtue of using an index, supports repeated types.
-   Here the `word 8` type is repeated but, depending on the index, it will use the first or third format.
-
-   We are still using words to directly encode indices
-                                               *)
-
-                                              Module SumTypeCodes3.
-
-                                                Let types:= [word 8:Type; word 16:Type; word 8:Type].
-                                                Definition formats : ilist (B := fun T => FormatM T ByteString) types
-                                                  := {{ format_word; format_word ; format_word }}.
-
-                                                Let invariants := ilist_constant_T types.
-                                                
-                                                Let view_fin {n} (f:Fin.t n):= f2n f < pow2 8.
-
-                                                Let invariant := (fun st : SumType types =>
-                                                                    view_fin (SumType_index types st) /\ ith invariants (SumType_index types st) (SumType_proj types st)).
-                                                
-                                                Let enc_dec : EncoderDecoderPair (format_IndexedSumType_word 8 formats) invariant.
-                                                Proof.
-                                                  unfold format_IndexedSumType_word.
-                                                  derive_encoder_decoder_pair.
-                                                  
-                                                  (* (*below are the instructions to do the automation step-by-step*)
-
-      econstructor.
-      - synthesize_aligned_encoder.
-      - start_synthesizing_decoder.
-        + normalize_format.
-          (* apply_IndexedSumTypeWord_Decoder_Correct 3 types.
-          {intuition
-              eauto 2 with data_inv_hints. }  *)
-          
-          apply_rules.
-        + cbv beta; synthesize_cache_invariant.
-        + cbv beta; unfold decode_nat, sequence_Decode; optimize_decoder_impl.
-        + cbv beta.
-          repeat align_decoders_step. *)
-                                                  
-
-                                                  
-                                                  (* align_decoders_step' *)
-                                                  (* AlignedDecodeSumTypeM *)
-                                                  
-                                                  Unshelve.
-                                                  (* This one is due to way `align_decoders_step`  deals with
-           `IterateBoundedIndex.prim_and`.
-           There is an already shelved `ilist` that slowly
-           decreases but obviously never gets completed (since the last goal doesn't depend).
-                                                   *)
-                                                  constructor.
-                                                Defined.
-                                                
-                                                Let encode := encoder_impl enc_dec.
-                                                
-                                                Let decode := decoder_impl enc_dec.
-                                                Print Assumptions decode.
-                                                
-                                              End SumTypeCodes3.
-
-
-                                              (** * Simple indexed sumtype (two formats)*)
-                                              (* | In this module we show different ways to encode the index.  Here
-   the index is encoded by a word (representing a label) which is
-   looked up in a vector to determine the index.
-                                               *)
-                                              Module SumTypeCodes_Enum.
-                                                
-                                                Let types:= [word 8:Type; word 16:Type].
-                                                
-                                                Definition formats : ilist (B := fun T => FormatM T ByteString) types
-                                                  := {{ format_word; format_word }}.
-                                                
-                                                Let invariants := ilist_constant_T types.
-                                                Let view_fin {n} (f:Fin.t n):= f2n f < pow2 8.
-                                                Let constT {T} (a:T):= True.
-                                                Let invariant := (fun st : SumType types =>  ((constant True) (SumType_index types st)) /\ ith invariants (SumType_index types st) (SumType_proj types st)).
-                                                
-                                                Let codes: Vector.t (word 8) 2:= [[ natToWord _ 42; natToWord _ 73 ]].
-                                                
-                                                Let enc_dec : EncoderDecoderPair (format_IndexedSumType_enum _ codes formats) invariant.
-                                                Proof.
-                                                  unfold format_IndexedSumType_enum.
-                                                  derive_encoder_decoder_pair.
-
-                                                  Unshelve.
-                                                  (* This one is due to way `align_decoders_step`  deals with
-           `IterateBoundedIndex.prim_and`.
-           There is an already shelved `ilist` that slowly
-           decreases but obviously never gets completed (since the last goal doesn't depend).
-                                                   *)
-                                                  constructor.
-                                                Defined.
-                                                
-                                                Let encode := encoder_impl enc_dec.
-                                                
-                                                Let decode := decoder_impl enc_dec.
-                                                
-                                              End SumTypeCodes_Enum.
-
-
-                                              (** * Motivating example*)
-                                              (* | Another example using Enum, which originally motivated this format.
-                                               *)
-                                              Module SumTypeCodes_Enum_Motivate.
-
-                                                (* This was the motivating example, which follows immidiately from out `format_IndexedSumType_enum` *)
-                                                Definition format_SumTypeCodes {m} {sz}
-                                                  (types : Vector.t Type (S m))
-                                                  (formatrs :
-                                                    ilist (B := fun T =>
-                                                                  T -> CacheFormat -> Comp (ByteString * CacheFormat)) types)
-                                                  (codes : Vector.t (word sz) (S m))
-                                                  (st : SumType types)
-                                                  : CacheFormat -> Comp (ByteString * CacheFormat):=
-                                                  format_IndexedSumType_enum m codes formatrs st.
-
-                                                (* Then we can show an example with that format *)
-                                                Let types:= [word 8:Type; word 16:Type; word 32:Type; word 16:Type; word 8:Type].
-                                                
-                                                Definition formats : ilist (B := fun T => FormatM T ByteString) types
-                                                  := {{ format_word; format_word; format_word; format_word; format_word }}.
-                                                
-                                                Let invariants := ilist_constant_T types.
-                                                Let view_fin {n} (f:Fin.t n):= f2n f < pow2 8.
-                                                Let constT {T} (a:T):= True.
-                                                Let invariant := (fun st : SumType types =>  ((constant True) (SumType_index types st)) /\ ith invariants (SumType_index types st) (SumType_proj types st)).
-
-                                                (* Let's index the entries using prime numbers *)
-                                                Let codes: Vector.t (word 8) 5:= [[ natToWord _ 2; natToWord _ 3; natToWord _ 5; natToWord _ 7; natToWord _ 11 ]].
-
-                                                Let enc_dec : EncoderDecoderPair (format_SumTypeCodes types formats codes) invariant.
-                                                Proof.
-                                                  unfold format_SumTypeCodes, format_IndexedSumType_enum.
-                                                  derive_encoder_decoder_pair.
-
-                                                  Unshelve.
-                                                  (* This one is due to way `align_decoders_step`  deals with
-           `IterateBoundedIndex.prim_and`.
-           There is an already shelved `ilist` that slowly
-           decreases but obviously never gets completed (since the last goal doesn't depend).
-                                                   *)
-                                                  constructor.
-                                                Defined.
-                                                
-                                              End SumTypeCodes_Enum_Motivate.
+  Let decode := decoder_impl enc_dec.
+  
+  
+  (* Quick goal to explore the decoder *)
+  Ltac remember_decoders:=
+    match goal with
+    | [ |- context [ListAlignedDecodeM (IndexedSumTypeAligneDecoder ?dec1 ?dec2) _] ] =>
+        remember dec2 as decoders
+    end.
+  
+  Goal forall m b result, decode m b  = result.
+    unfold decode,AlignedDecoderPermutation, AlignedSortList.
+    intros; remember_decoders.
+  Abort.
+  
+End AllEqualPermutation.
